opentheory/examples/all.ml
@@ -4,22 +4,29 @@
 
 start_logging ();;
 
+(* Natural number division *)
 loads "opentheory/examples/divides.ml";;
 loads "opentheory/examples/gcd.ml";;
 loads "opentheory/examples/prime.ml";;
 
+(* Modular arithmetic *)
 loads "opentheory/examples/modular.ml";;
+
+(* Finite fields GF(p) *)
 loads "opentheory/examples/gfp.ml";;
 
+(* Bit-vectors *)
 loads "opentheory/examples/word.ml";;
 loads "opentheory/examples/byte.ml";;
 loads "opentheory/examples/word10.ml";;
 loads "opentheory/examples/word12.ml";;
 loads "opentheory/examples/word16.ml";;
 
+(* Simple stream parsers *)
 loads "opentheory/examples/parser.ml";;
 loads "opentheory/examples/char.ml";;
 
+(* Memory safety for the H interface *)
 loads "opentheory/examples/h.ml";;
 
 stop_logging ();;
